Translation/Ty.lean
@@ -22,6 +22,7 @@ def Surface.Ty.translate: Surface.Ty -> Core.Ty
 | .var x => .var x
 | .global x => .global x
 | .arrow a b => .arrow (a.translate) (b.translate)
+| .then a b => .arrow (a.translate) (b.translate)
 | .app a b => .app (a.translate) (b.translate)
 | .all k p =>
   .all k.translate (p.translate)
@@ -38,3 +39,28 @@ def Subst.Surface.Ty.translate (σ : Subst Surface.Ty) : Subst Core.Ty :=
   | .re x => .re x
   | .su T => .su (T.translate)) <$> σ
 notation "⟦" σ "⟧" => Subst.Surface.Ty.translate σ
+
+
+inductive Surface.Translation.Ty (G : Surface.GlobalEnv) (G' : Core.GlobalEnv) :
+  Surface.KindEnv -> Surface.Ty -> Surface.Kind ->
+  Core.KindEnv -> Core.Ty -> Core.Kind -> Prop where
+| var {Δ : Surface.KindEnv} :
+  Δ[i]? = some K ->
+  Δ'[i]? = some K.translate ->
+  Translation.Ty G G' Δ t`#i K Δ' t#i K.translate
+| arrow :
+  Translation.Ty G G' Δ A `★ Δ' A' ★ ->
+  Translation.Ty G G' Δ B K Δ' B' K.translate ->
+  Translation.Ty G G' Δ (A `-:> B) `★ Δ' (A' -:> B') ★
+| «then» :
+  Translation.Ty G G' Δ A `◯ Δ' A' ◯ ->
+  Translation.Ty G G' Δ B K Δ' B' K.translate ->
+  Translation.Ty G G' Δ (A `=:> B) `★ Δ' (A' -:> B') ★
+| app :
+  Translation.Ty G G' Δ A (.arrow K1 K2) Δ' A' (Surface.Kind.arrow K1 K2).translate ->
+  Translation.Ty G G' Δ B K1 Δ' B' K1.translate ->
+  Translation.Ty G G' Δ (A `• B) K2 Δ' (A' • B') K2.translate
+| all :
+  Translation.Ty G G' Δ A K Δ' A' K.translate ->
+  Translation.Ty G G' (K::Δ) B `★ (K.translate::Δ') B' ★ ->
+  Translation.Ty G G' Δ (`∀[K]B) `★ Δ' (∀[K.translate] B') ★
