Surface.lean
@@ -1,2 +1,3 @@
 import Surface.Ty
 import Surface.Term
+import Surface.Metatheory
