Surface/Metatheory.lean
@@ -1,0 +1,4 @@
+import Surface.Metatheory.Rename
+import Surface.Metatheory.Substitution
+import Surface.Metatheory.GlobalWf
+import Surface.Metatheory.Inversion
